fix definition of wf_subst

Term.thy
@@ -56,14 +56,14 @@ qed auto
 
 lemma embed_msg_of_term [simp]: "wf_term arity x \<Longrightarrow> embed (msg_of_term x) = x"
 proof(induction rule:wf_term.induct)
-case (1 uu)
+case (wf_term_intro_var uu)
 then show ?case by auto
 next
-case (2 l f)
+case (wf_term_intro_fun l f)
   then show ?case
 (* arity goes up to 2 so pattern match on up to 2 elements of l*)
   proof(cases f;cases l;(cases "tl l")?)
-  qed(auto simp add:"2.IH")
+  qed(auto simp add:"wf_term_intro_fun.IH")
 qed
 
 (* (c) : transfer of various functions via embedding 
@@ -78,17 +78,44 @@ fun embed_subst :: "subst_msg \<Rightarrow> (var \<Rightarrow> msg_term)" where
 "embed_subst s = embed o s"
 fun subst_from_embed :: "(var \<Rightarrow> msg_term) \<Rightarrow> subst_msg"  where
 "subst_from_embed s = msg_of_term o s"
+
 lemma embed_subst_from_embed [simp]: "wf_subst arity x \<Longrightarrow> embed \<circ> (msg_of_term \<circ> x) = x"
-  by(auto)
+proof(induction rule:wf_subst.induct)
+  case (1 \<sigma>)
+  then show ?case by(auto simp add:fun_eq_iff)
+qed
 
 (* sapply *)
 definition sapply_msg :: "subst_msg \<Rightarrow> msg \<Rightarrow> msg" where
 "sapply_msg s m = msg_of_term (sapply (embed_subst s) (embed m))"
 
+lemma sapply_msg_msg_of_term [simp]:
+"wf_subst arity s \<Longrightarrow> sapply_msg (msg_of_term \<circ> s)= msg_of_term o (sapply s) o embed"
+  by(auto simp add:sapply_msg_def)
+
 (* unifies *)
 type_synonym eq_msg = "msg \<times> msg"
 fun embed_eq :: "eq_msg \<Rightarrow> (symbol, var) equation" where
 "embed_eq (a, b) = (embed a, embed b)"
+fun eq_from_embed:: "(symbol, var) equation \<Rightarrow> eq_msg" where
+"eq_from_embed (a, b) = (msg_of_term a, msg_of_term b)"
+
+lemma wf_embed_eq [simp]:"wf_eq arity (embed_eq e)" by(cases e; auto intro:wf_eq.intros)
+lemma wf_embed_eqs [simp]:"wf_eqs arity (map embed_eq l)"
+proof(rule wf_eqs.intros)
+qed simp
+lemma "embed_eq_eq_from_embed" [simp]: "wf_eq arity e \<Longrightarrow> embed_eq (eq_from_embed e) = e"
+proof(cases e)
+  case (Pair a b)
+  assume "wf_eq arity e"
+  then have x:"wf_eq arity (a, b)" by(simp add:Pair)
+  then have "wf_term arity a" by(cases rule:wf_eq.cases; auto)
+  moreover from x have "wf_term arity b" by(cases rule:wf_eq.cases; auto)
+  ultimately show "embed_eq (eq_from_embed e) = e"
+    by(auto simp add:Pair)
+qed
+lemma "eq_from_embed_embed_eq" [simp]: "eq_from_embed (embed_eq e) = e"
+  by(cases e;auto)
 
 definition unifies_msg :: "subst_msg \<Rightarrow> eq_msg \<Rightarrow> bool" where
   "unifies_msg s eq = unifies (embed_subst s) (embed_eq eq)"
@@ -122,6 +149,63 @@ proof -
     apply(rule unify_return)
   apply(simp only:xdef `wf_subst arity x` embed_subst_from_embed)
     done
+qed
+
+(* (f) *)
+fun fv_eq_msg:: "eq_msg \<Rightarrow> var set" where
+"fv_eq_msg (a, b) = fv_msg a \<union> fv_msg b"
+definition fv_eqs_msg:: "eq_msg list \<Rightarrow> var set" where
+"fv_eqs_msg l = fv_eqs (map embed_eq l)"
+
+lemma fv_eqs_msg_fv_msg: "fv_eqs_msg l = (\<Union> x \<in> set l. fv_eq_msg x)"
+  by(auto simp add:fv_eqs_msg_def fv_msg_def)
+
+fun sapply_eq_msg:: "subst_msg \<Rightarrow> eq_msg \<Rightarrow> eq_msg" where
+"sapply_eq_msg s (a, b) = (sapply_msg s a, sapply_msg s b)"
+definition sapply_eqs_msg:: "subst_msg \<Rightarrow> eq_msg list \<Rightarrow> eq_msg list" where
+"sapply_eqs_msg s l = map eq_from_embed (sapply_eqs (embed_subst s) (map embed_eq l))"
+
+lemma "sapply_eqs_msg s l = map (sapply_eq_msg s) l"
+  by(auto simp add:sapply_eqs_msg_def sapply_msg_def)
+
+definition sdom_msg:: "subst_msg \<Rightarrow> var set" where
+"sdom_msg s = sdom (embed_subst s)"
+definition svran_msg:: "subst_msg \<Rightarrow> var set" where
+"svran_msg s = svran (embed_subst s)"
+
+lemma l3_msg:
+  fixes \<sigma> :: "subst_msg" 
+    and l :: "eq_msg list"
+  assumes "unify_msg l = Some s"
+  shows "fv_eqs_msg (sapply_eqs_msg s l) \<subseteq> fv_eqs_msg l"
+    and "sdom_msg s \<subseteq> fv_eqs_msg l"
+    and "svran_msg s \<subseteq> fv_eqs_msg l"
+    and "sdom_msg s \<inter> svran_msg s = {}"
+proof -
+  let ?l' = "map embed_eq l"
+  from assms obtain s'
+    where return:"unify ?l' = Some s'" and sdef:"s = msg_of_term \<circ> s'"
+    by(auto simp add:unify_msg_def sdom_msg_def split:option.split_asm)
+  have wf:"wf_eqs arity ?l'" by simp
+  from return  and this have wfs:"wf_subst arity s'" by(rule wf_subst_unify)
+
+(* goal 1*)
+  from return have "fv_eqs (sapply_eqs s' ?l') \<subseteq> fv_eqs ?l'" by(rule 3)
+  then  show  "fv_eqs_msg (sapply_eqs_msg s l) \<subseteq> fv_eqs_msg l"
+    by(simp add:sapply_eqs_msg_def wf_eq_sapply_eq fv_eqs_msg_def sdef wf wfs)
+(*goal 2*)
+  from return have "sdom s' \<subseteq> fv_eqs ?l'" by(rule 3)
+  then show "sdom_msg s \<subseteq> fv_eqs_msg l"
+    by(simp add:sdom_msg_def fv_eqs_msg_def sdef wfs)
+
+(* goal 3*)
+  from return have "svran s' \<subseteq> fv_eqs ?l'" by(rule 3)
+  then show "svran_msg s \<subseteq> fv_eqs_msg l"
+    by(simp add:svran_msg_def fv_eqs_msg_def sdef wfs)
+      (*goal 4*)
+  from return have "sdom s' \<inter> svran s' = {}" by(rule 3)
+  then show "sdom_msg s \<inter> svran_msg s = {}"
+    by(simp add:sdom_msg_def svran_msg_def fv_eqs_msg_def sdef wfs)
 qed
 
 end
